Veritas.SeqAux.fsti
@@ -28,7 +28,7 @@ val lemma_suffix_index (#a:Type) (s:seq a) (i:nat{i <= length s}) (j:nat{j < i})
         (ensures (index (suffix s i) j == index s (length s - i + j)))
 
 (* Subsequence of s obtained by applying a filter *)
-val filter (#a:eqtype) (f:a -> bool) (s:seq a): Tot (seq (x:a{f x}))
+val filter (#a:eqtype) (f:a -> bool) (s:seq a): Tot (seq a)
 
 (* Mapping from original seq to filtered subseq for satisfying indexes *)
 val filter_index_map (#a:eqtype) (f:a -> bool) (s:seq a) (i:seq_index s{f (index s i)}):
@@ -44,6 +44,12 @@ val filter_index_map_monotonic (#a:eqtype) (f:a -> bool) (s:seq a)
 val filter_index_inv_map (#a:eqtype) (f:a -> bool) (s:seq a) 
   (i:seq_index (filter f s)): 
   Tot (j:seq_index s{f (index s j) /\ filter_index_map f s j = i})
+
+(* Every element of the filter satisfies the filter predicate *)
+val lemma_filter_sat (#a:eqtype) (f:a -> bool) (s:seq a) (i:seq_index (filter f s)):
+  Lemma (requires (True))
+        (ensures (f (index (filter f s) i)))
+
 
 (* The index of the last entry that satisfies a given property *)
 val last_index_opt (#a:eqtype) (f:a -> bool) (s:seq a):
